implement simple tensor core matmul (plus C)

src/lib/poly/gemm/Kuiper.Poly.GEMM.TensorCore.fst
@@ -25,6 +25,7 @@ open Kuiper.VArray {
   varray_pts_to_cell
 }
 open Kuiper.TensorCore
+open Kuiper.Float16
 open Kuiper.Matrix.Tiling
 
 (* Description of shared memory used in this kernel. *)
@@ -40,135 +41,152 @@ let shmems_desc
 
 unfold
 let bid_y
-  (rows cols : nat)
-  (bm : nat {bm > 0 /\ bm /? rows})
-  (bn : nat {bn > 0 /\ bn /? cols})
-  (bid : natlt (rows/bm * (cols/bn)))
-  : natlt (rows/bm)
+  (rows cols : erased nat)
+  (bm : erased nat {bm > 0 /\ bm /? rows})
+  (bn : erased nat {bn > 0 /\ bn /? cols})
+  (bid : enatlt (rows/bm * (cols/bn)))
+  : enatlt (rows/bm)
   =
     bid / (cols/bn)
 
 unfold
 let bid_x
-  (rows cols : nat)
-  (bm : nat {bm > 0 /\ bm /? rows})
-  (bn : nat {bn > 0 /\ bn /? cols})
-  (bid : natlt (rows/bm * (cols/bn)))
-  : natlt (cols/bn)
+  (rows cols : erased nat)
+  (bm : erased nat {bm > 0 /\ bm /? rows})
+  (bn : erased nat {bn > 0 /\ bn /? cols})
+  (bid : enatlt (rows/bm * (cols/bn)))
+  : enatlt (cols/bn)
   =
   bid % (cols/bn)
 
 unfold
 let tid_y
-  (bm bn : nat)
-  (tm : nat {tm > 0 /\ tm /? bm})
-  (tn : nat {tn > 0 /\ tn /? bn})
-  (tid : natlt (bm/tm * (bn/tn)))
-  : natlt (bm/tm)
+  (bm bn : erased nat)
+  (tm : erased nat {tm > 0 /\ tm /? bm})
+  (tn : erased nat {tn > 0 /\ tn /? bn})
+  (tid : enatlt (bm/tm * (bn/tn)))
+  : enatlt (bm/tm)
   =
     tid / (bn/tn)
 
 unfold
 let tid_x
-  (bm bn : nat)
-  (tm : nat {tm > 0 /\ tm /? bm})
-  (tn : nat {tn > 0 /\ tn /? bn})
-  (tid : natlt (bm/tm * (bn/tn)))
-  : natlt (bn/tn)
+  (bm bn : erased nat)
+  (tm : erased nat {tm > 0 /\ tm /? bm})
+  (tn : erased nat {tn > 0 /\ tn /? bn})
+  (tid : enatlt (bm/tm * (bn/tn)))
+  : enatlt (bn/tn)
   =
     tid % (bn/tn)
 
 inline_for_extraction noextract
 instance concrete_sz_1 : concrete_sz 1 = { x = 1sz }
 
+inline_for_extraction noextract
 let block_tile
   (#et : Type0) {| scalar et |}
   (#rows #cols : erased nat)
   (#lC : mlayout rows cols)
   (gC : gpu_matrix et lC)
-  (bm : szp{bm /? rows})
-  (bn : szp{bn /? cols})
+  (bm : erased nat{bm > 0 /\ bm /? rows})
+  (bn : erased nat{bn > 0 /\ bn /? cols})
   (bid : enatlt (rows/bm * (cols/bn)))
-  : gpu_matrix et
-      (subtile_layout lC bm bn
-        (bid_y rows cols (hide (SZ.v bm)) (hide (SZ.v bn)) bid)
-        (bid_x rows cols (hide (SZ.v bm)) (hide (SZ.v bn)) bid))
+  : Tot (gpu_matrix et
+          (subtile_layout lC bm bn
+            (bid_y rows cols bm bn bid)
+            (bid_x rows cols bm bn bid)))
   =
-    gpu_matrix_subtile gC (hide (SZ.v bm)) (hide (SZ.v bn))
+    gpu_matrix_subtile gC bm bn
       (bid_y rows cols bm bn bid) (bid_x rows cols bm bn bid)
 
+inline_for_extraction noextract
 let thread_tile
   (#et : Type0) {| scalar et |}
-  (#bm #bn : sz)
+  (#bm #bn : erased nat)
   (#lC_bt : mlayout bm bn)
   (gC_bt : gpu_matrix et lC_bt)
-  (tm : szp{tm /? bm})
-  (tn : szp{tn /? bn})
+  (tm : erased nat{tm > 0 /\ tm /? bm})
+  (tn : erased nat{tn > 0 /\ tn /? bn})
   (tid : enatlt (bm/tm * (bn/tn)))
-  : gpu_matrix et
-      (subtile_layout lC_bt tm tn
-        (tid_y bm bn tm tn tid) (tid_x bm bn tm tn tid))
+  : Tot (gpu_matrix et
+          (subtile_layout lC_bt tm tn
+            (tid_y bm bn tm tn tid) (tid_x bm bn tm tn tid)))
   =
-   gpu_matrix_subtile gC_bt (hide (SZ.v tm)) (hide (SZ.v tn))
+   gpu_matrix_subtile gC_bt tm tn
     (tid_y bm bn tm tn tid) (tid_x bm bn tm tn tid)
 
 let own_thread_tile
   (#et : Type0) {| scalar et |}
-  (#rows #cols : erased nat)
+  // Since this is an slprop, I would like to not erase the nat.
+  // Unfortunately, when unfolding own_thread_tile, after passing
+  // a (reveal x) as argument, this leads to (reveal (hide (reveal x)))
+  // which creates problems with type equalities.
+  (#rows : erased nat)
+  (#cols : nat)
   (#lC : mlayout rows cols)
   (gC : gpu_matrix et lC)
-  (bm : szp{bm /? rows})
-  (bn : szp{bn /? cols})
-  (tm : szp{tm /? bm})
-  (tn : szp{tn /? bn})
-  (bid : enatlt ((rows/bm) * (cols/bn)))
-  (tid : enatlt (bm/tm * (bn/tn)))
+  (bm : nat{bm > 0 /\ bm /? rows})
+  (bn : nat{bn > 0 /\ bn /? cols})
+  (tm : nat{tm > 0 /\ tm /? bm})
+  (tn : nat{tn > 0 /\ tn /? bn})
+  (bid : natlt ((rows/bm) * (cols/bn)))
+  (tid : natlt (bm/tm * (bn/tn)))
   : slprop
   =
     exists* em.
       gpu_matrix_pts_to
         (thread_tile (block_tile gC bm bn bid) tm tn tid) em
 
+// TODO look again at why we cannot use nats here instead of sizet
 unfold
 let kpre1
-  (#et : Type0) {| scalar et |}
-  (comb : binop et)
+  (#et_ab #et_c : Type0) {| scalar et_ab, scalar et_c |}
   (#rows #shared #cols : szp)
   (#lA : mlayout rows shared)
   (#lB : mlayout shared cols)
   (#lC : mlayout rows cols)
-  (gA : gpu_matrix et lA)
-  (eA : ematrix et rows shared)
-  (gB : gpu_matrix et lB)
-  (eB : ematrix et shared cols)
-  (gC : gpu_matrix et lC)
+  (gA : gpu_matrix et_ab lA)
+  (eA : ematrix et_ab rows shared)
+  (gB : gpu_matrix et_ab lB)
+  (eB : ematrix et_ab shared cols)
+  (gC : gpu_matrix et_c lC)
   (bm : szp{bm /? rows})
   (bn : szp{bn /? cols})
   (bk : szp{bk /? shared})
   (tm : szp{tm /? bm})
   (tn : szp{tn /? bn})
+  (tk : szp{tk /? bk})
   (fA fB : perm)
   (bid : enatlt (rows/bm * (cols/bn)))
   (tid : enatlt (bm/tm * (bn/tn)))
   : slprop
   =
+  pure (SZ.fits (rows * shared)) **
+  pure (SZ.fits (shared * cols)) **
+  pure (valid_frag_et_dims et_ab FragA tm tn tk) **
+  pure (valid_frag_et_dims et_ab FragB tm tn tk) **
+  pure (valid_frag_et_dims et_c FragAcc tm tn tk) **
+  pure (valid_frag_et_comb et_ab et_c) **
+  // could be added if it wasn't trivially true
+  // pure (valid_frag_et_comb et et) **
   gA |-> Frac (fA /. (rows/tm * (cols/tn))) eA **
   gB |-> Frac (fB /. (rows/tm * (cols/tn))) eB **
-  own_thread_tile gC bm bn tm tn bid tid
+  // see comment at own_thread_tile for why we explicitly
+  // have to convert (so that the reaveal coercion can kick in)
+  own_thread_tile gC (SZ.v bm) (SZ.v bn) (SZ.v tm) (SZ.v tn) bid tid
 
 unfold
 let kpost1
-  (#et : Type0) {| scalar et |}
-  (comb : binop et)
+  (#et_ab #et_c : Type0) {| scalar et_ab, scalar et_c |}
   (#rows #shared #cols : szp)
   (#lA : mlayout rows shared)
   (#lB : mlayout shared cols)
   (#lC : mlayout rows cols)
-  (gA : gpu_matrix et lA)
-  (eA : ematrix et rows shared)
-  (gB : gpu_matrix et lB)
-  (eB : ematrix et shared cols)
-  (gC : gpu_matrix et lC)
+  (gA : gpu_matrix et_ab lA)
+  (eA : ematrix et_ab rows shared)
+  (gB : gpu_matrix et_ab lB)
+  (eB : ematrix et_ab shared cols)
+  (gC : gpu_matrix et_c lC)
   (bm : szp{bm /? rows})
   (bn : szp{bn /? cols})
   (bk : szp{bk /? shared})
@@ -181,15 +199,15 @@ let kpost1
   =
   gA |-> Frac (fA /. (rows/tm * (cols/tn))) eA **
   gB |-> Frac (fB /. (rows/tm * (cols/tn))) eB **
-  own_thread_tile gC bm bn tm tn bid tid
+  own_thread_tile gC (SZ.v bm) (SZ.v bn) (SZ.v tm) (SZ.v tn) bid tid
 
 let own_shmem_cell
   (#et : Type0)
-  (#rows #cols : erased nat)
+  (#rows #cols : nat)
   (#lm : mlayout rows cols)
   (sm : gpu_matrix et lm)
-  (i : enatlt rows)
-  (j : enatlt cols)
+  (i : natlt rows)
+  (j : natlt cols)
   : slprop
   = exists* v. gpu_matrix_pts_to_cell sm i j v
 
@@ -285,8 +303,8 @@ let barrier_p
   : B.barrier_side nthr =
   fun it tid ->
     if even it then
-      exists* (x : ematrix _ _ _). m1 |-> Frac (1.0R /. nthr) x **
-      exists* (x : ematrix _ _ _). m2 |-> Frac (1.0R /. nthr) x
+      (exists* (x : ematrix _ _ _). m1 |-> Frac (1.0R /. nthr) x) **
+      (exists* (x : ematrix _ _ _). m2 |-> Frac (1.0R /. nthr) x)
     else
       own_tile_stride_cells m1 nthr tid **
       own_tile_stride_cells m2 nthr tid
@@ -323,67 +341,62 @@ let barrier_tok
 
 unfold
 let kpre
-  (#et : Type0) {| scalar et |}
-  (comb : binop et)
+  (#et_ab #et_c : Type0) {| scalar et_ab, scalar et_c |}
   (#rows #shared #cols : szp)
   (#lA : mlayout rows shared)
   (#lB : mlayout shared cols)
   (#lC : mlayout rows cols)
-  (gA : gpu_matrix et lA)
-  (eA : ematrix et rows shared)
-  (gB : gpu_matrix et lB)
-  (eB : ematrix et shared cols)
-  (gC : gpu_matrix et lC)
+  (gA : gpu_matrix et_ab lA)
+  (eA : ematrix et_ab rows shared)
+  (gB : gpu_matrix et_ab lB)
+  (eB : ematrix et_ab shared cols)
+  (gC : gpu_matrix et_c lC)
   (bm : szp{bm /? rows})
   (bn : szp{bn /? cols})
   (bk : szp{bk /? shared})
   (#_: squash (SZ.fits (bm * bk) /\ SZ.fits (bk * bn)))
-  (slA : full_mlayout bm bk)
-  (slB : full_mlayout bk bn)
   (tm : szp{tm /? bm})
   (tn : szp{tn /? bn})
+  (tk : szp{tk /? bk})
   (fA fB : perm)
-  (sh : c_shmems (shmems_desc et bm bn bk))
+  (sh : c_shmems (shmems_desc et_ab bm bn bk))
   (bid : natlt (rows/bm * (cols/bn)))
   (tid : natlt (bm/tm * (bn/tn)))
   : slprop
   =
-  kpre1 comb gA eA gB eB gC bm bn bk tm tn fA fB bid tid **
+  kpre1 gA eA gB eB gC bm bn bk tm tn tk fA fB bid tid **
   exists* (x : seq _). fst sh |-> Frac (1.0R /. (bm/tm * (bn/tn))) x **
   exists* (x : seq _). fst (snd sh) |-> Frac (1.0R /. (bm/tm * (bn/tn))) x **
-  barrier_tok slA slB (fst sh) (fst (snd sh)) 0 (bm/tm * (bn/tn)) tid
+  barrier_tok (R.row_major bm bk) (R.row_major bk bn) (fst sh) (fst (snd sh)) 0 (bm/tm * (bn/tn)) tid
 
 unfold
 let kpost
-  (#et : Type0) {| scalar et |}
-  (comb : binop et)
+  (#et_ab #et_c : Type0) {| scalar et_ab, scalar et_c |}
   (#rows #shared #cols : szp)
   (#lA : mlayout rows shared)
   (#lB : mlayout shared cols)
   (#lC : mlayout rows cols)
-  (gA : gpu_matrix et lA)
-  (eA : ematrix et rows shared)
-  (gB : gpu_matrix et lB)
-  (eB : ematrix et shared cols)
-  (gC : gpu_matrix et lC)
+  (gA : gpu_matrix et_ab lA)
+  (eA : ematrix et_ab rows shared)
+  (gB : gpu_matrix et_ab lB)
+  (eB : ematrix et_ab shared cols)
+  (gC : gpu_matrix et_c lC)
   (bm : szp{bm /? rows})
   (bn : szp{bn /? cols})
   (bk : szp{bk /? shared})
   (#_: squash (SZ.fits (bm * bk) /\ SZ.fits (bk * bn)))
-  (slA : full_mlayout bm bk)
-  (slB : full_mlayout bk bn)
   (tm : szp{tm /? bm})
   (tn : szp{tn /? bn})
   (fA fB : perm)
-  (sh : c_shmems (shmems_desc et bm bn bk))
+  (sh : c_shmems (shmems_desc et_ab bm bn bk))
   (bid : natlt (rows/bm * (cols/bn)))
   (tid : natlt (bm/tm * (bn/tn)))
   : slprop
   =
-  kpost1 comb gA eA gB eB gC bm bn bk tm tn fA fB bid tid **
+  kpost1 (* comb *) gA eA gB eB gC bm bn bk tm tn fA fB bid tid **
   exists* (x : seq _). fst sh |-> Frac (1.0R /. (bm/tm * (bn/tn))) x **
   exists* (x : seq _). fst (snd sh) |-> Frac (1.0R /. (bm/tm * (bn/tn))) x **
-  barrier_tok slA slB (fst sh) (fst (snd sh)) (2 * (shared/bk)) (bm/tm * (bn/tn)) tid
+  barrier_tok (R.row_major bm bk) (R.row_major bk bn) (fst sh) (fst (snd sh)) (2 * (shared/bk)) (bm/tm * (bn/tn)) tid
 
 inline_for_extraction noextract
 fn populate_shmem
@@ -434,29 +447,30 @@ fn populate_shmem
 
 inline_for_extraction noextract
 fn subproducts_tc
-  (* TODO restrict et to valid types only *)
-  // (#et : Type0) {| scalar et |}
+  (#et_ab #et_acc : Type0)
+  {| scalar et_ab, scalar et_acc |}
   (bm bn bk: szp)
   (tm : szp{tm /? bm})
   (tn : szp{tn /? bn})
   (tk : szp{tk /? bk})
-  (aFrag : fragment half FragA tm tn tk FragLRM)
-  (#vaFrag : ematrix half tm tk)
-  (bFrag : fragment half FragB tm tn tk FragLRM)
-  (#vbFrag : ematrix half tk tn)
-  (accumFrag : fragment half FragAccum tm tn tk FragLAccum)
-  (#vaccumFrag : ematrix half tm tn)
-  (gA : gpu_matrix half (R.row_major bm bk))
-  (gB : gpu_matrix half (R.row_major bk bn))
-  (#eA : ematrix half bm bk)
-  (#eB : ematrix half bk bn)
-  (#f : perm)
+  (aFrag : fragment et_ab FragA tm tn tk FragLRM)
+  (#vaFrag : ematrix et_ab tm tk)
+  (bFrag : fragment et_ab FragB tm tn tk FragLRM)
+  (#vbFrag : ematrix et_ab tk tn)
+  (accumFrag : fragment et_acc FragAcc tm tn tk FragLAcc)
+  (#vaccumFrag : ematrix et_acc tm tn)
+  (gA : gpu_matrix et_ab (R.row_major bm bk))
+  (gB : gpu_matrix et_ab (R.row_major bk bn))
+  (#eA : ematrix et_ab bm bk)
+  (#eB : ematrix et_ab bk bn)
+  (#fA #fB : perm)
   (arow: szlt (bm/tm))
   (bcol : szlt (bn/tn))
   preserves
     gpu **
-    gA |-> Frac f eA **
-    gB |-> Frac f eB
+    pure (valid_frag_et_comb et_ab et_acc) **
+    gA |-> Frac fA eA **
+    gB |-> Frac fB eB
   requires
     aFrag |-> vaFrag **
     bFrag |-> vbFrag **
@@ -470,8 +484,8 @@ fn subproducts_tc
   let mut dotIdx : sz = 0sz;
   while (SZ.(!dotIdx <^ (bk/^tk)))
     invariant
-      exists* (vdotIdx : sz{vdotIdx <= (bk/^tk)}) (vaFrag : ematrix half tm tk)
-        (vbFrag : ematrix half tk tn) (vaccumFrag : ematrix half tm tn).
+      exists* (vdotIdx : sz{vdotIdx <= (bk/^tk)}) (vaFrag : ematrix et_ab tm tk)
+        (vbFrag : ematrix et_ab tk tn) (vaccumFrag : ematrix et_acc tm tn).
         dotIdx |-> vdotIdx **
         aFrag |-> vaFrag **
         bFrag |-> vbFrag **
@@ -493,11 +507,11 @@ fn subproducts_tc
     mma_sync' aFrag bFrag accumFrag;
 
     with etA.
-      assert (gpu_matrix_pts_to a_tile #f etA);
-      Pulse.Lib.Trade.elim_trade (a_tile |-> Frac f etA) (gA |-> Frac f eA);
+      assert (gpu_matrix_pts_to a_tile #fA etA);
+      Pulse.Lib.Trade.elim_trade (a_tile |-> Frac fA etA) (gA |-> Frac fA eA);
     with etB.
-      assert (gpu_matrix_pts_to b_tile #f etB);
-      Pulse.Lib.Trade.elim_trade (b_tile |-> Frac f etB) (gB |-> Frac f eB);
+      assert (gpu_matrix_pts_to b_tile #fB etB);
+      Pulse.Lib.Trade.elim_trade (b_tile |-> Frac fB etB) (gB |-> Frac fB eB);
 
     dotIdx := !dotIdx +^ 1sz;
   };
@@ -507,197 +521,226 @@ fn subproducts_tc
 
 inline_for_extraction noextract
 fn epilogue
-  // (#et : Type0) {| scalar et |}
+  (#et : Type0) {| scalar et |}
   // (comb : binop et)
-  (#rows #cols : nat)
+
+  // rows should be an erased nat because not concerete value is required, but
+  // using erased nats here leads to very confusing reveals when calling mma_store
+  //  (maybe due to inferred type class instances?)
+  // making it a size because otherwise a nat would be extracted
+  (#rows : erased nat)
+  // cols is concretized so using size is fine I think
+  (#cols : sz)
   (bm : szp{bm /? rows})
   (bn : szp{bn /? cols})
   (tm : szp{tm /? bm})
   (tn : szp{tn /? bn})
-  (#tk : nat)
-  (accumFrag : fragment half FragAccum tm tn tk FragLAccum)
-  (gC : gpu_matrix half (R.row_major rows cols))
-  // (#_ : squash (SZ.fits (bm/tm * (bn/tn))))
+  (#tk : erased nat)
+  (accumFrag : fragment et FragAcc tm tn tk FragLAcc)
+  (gC : gpu_matrix et (R.row_major rows cols))
   (bid : szlt (rows/bm * (cols/bn)))
   (tid : szlt (bm/tm * (bn/tn)))
   requires
     gpu **
-    own_thread_tile gC bm bn tm tn (hide (SZ.v bid)) (hide (SZ.v tid)) **
+    // see comment in own_thread_tile for why SZ.v
+    own_thread_tile gC bm bn tm tn bid tid **
     (exists* vaccumFrag.
       accumFrag |-> vaccumFrag)
   ensures
     gpu **
-    own_thread_tile gC bm bn tm tn (hide (SZ.v bid)) (hide (SZ.v tid)) **
+    own_thread_tile gC bm bn tm tn bid tid **
     (exists* vaccumFrag.
       accumFrag |-> vaccumFrag)
 {
-  unfold own_thread_tile gC bm bn tm tn (hide (SZ.v bid)) (hide (SZ.v tid));
+  unfold own_thread_tile gC bm bn tm tn bid tid;
 
-  (* Only create a tile in gC and write the accumulator values. In this version the input from the gC
+  (* Only create a tile in gC and write the accumulator values. In this version the input from gC
      was added by loading the tile into the accumulator before any other computations *)
-  let t_tile = thread_tile (block_tile gC bm bn (hide (SZ.v bid))) tm tn (hide (SZ.v tid));
-  assert (rewrites_to t_tile (thread_tile (block_tile gC bm bn (hide (SZ.v bid))) tm tn (hide (SZ.v tid))));
+  let t_tile = thread_tile (block_tile gC (SZ.v bm) (SZ.v bn) (hide (SZ.v bid)))
+    (SZ.v tm) (SZ.v tn) (hide (SZ.v tid));
+  assert (rewrites_to t_tile (thread_tile (block_tile gC (SZ.v bm) (SZ.v bn) (hide (SZ.v bid)))
+    (SZ.v tm) (SZ.v tn) (hide (SZ.v tid))));
 
-  // mma_store accumFrag gC;
+  // from looking at the type of mma_store, it is not clear that cols mut be concretizable
+  // 1. know that strided_row_major needs concrete sizes
+  // 2. search the code base for the appropriate instance and see which of the arguments
+  //   must be concretizable
+  // 3. figure out which expression is which argument and make concretizable accordingly
+  mma_store accumFrag t_tile;
 
   // rewrite each t_tile as thread_tile (block_tile gC bm bn bid) tm tn tid;
-  fold own_thread_tile gC bm bn tm tn (hide (SZ.v bid)) (hide (SZ.v tid));
+  fold own_thread_tile gC bm bn tm tn bid tid;
   ()
 }
 
-// inline_for_extraction noextract
-// fn kf
-//   (#et : Type0) {| scalar et |}
-//   (comb : binop et)
-//   (#rows #shared #cols : szp)
-//   (#lA : mlayout rows shared)
-//   (#lB : mlayout shared cols)
-//   (#lC : mlayout rows cols)
-//   {| clayout lA, clayout lB, clayout lC |}
-//   (gA : gpu_matrix et lA)
-//   (#eA : ematrix et rows shared)
-//   (gB : gpu_matrix et lB)
-//   (#eB : ematrix et shared cols)
-//   (gC : gpu_matrix et lC)
-//   (bm : szp{bm /? rows})
-//   (bn : szp{bn /? cols})
-//   (bk : szp{bk /? shared})
-//   (#_: squash (SZ.fits (bm * bk) /\ SZ.fits (bk * bn)))
-//   (slA : full_mlayout bm bk)
-//   (slB : full_mlayout bk bn)
-//   {| clayout slA, clayout slB |}
-//   (tm : szp{tm /? bm})
-//   (tn : szp{tn /? bn})
-//   (tk : szp{tk /? bk})
-//   (#_ : squash (SZ.fits (bm*bk + bm/tm*(bn/tn))))
-//   (#_ : squash (SZ.fits (bk*bn + bm/tm*(bn/tn))))
-//   (#fA #fB : perm)
-//   (sh : c_shmems (shmems_desc et bm bn bk))
-//   (bid : szlt (rows/bm * (cols/bn)))
-//   (tid : szlt (bm/tm * (bn/tn)))
-//   ()
-//   requires
-//     gpu **
-//     kpre comb gA eA gB eB gC bm bn bk slA slB tm tn fA fB sh bid tid **
-//     thread_id (bm/tm * (bn/tn)) tid **
-//     block_id (rows/bm * (cols/bn)) bid
-//   ensures
-//     gpu **
-//     kpost comb gA eA gB eB gC bm bn bk slA slB tm tn fA fB sh bid tid **
-//     thread_id (bm/tm * (bn/tn)) tid **
-//     block_id (rows/bm * (cols/bn)) bid
-// {
-//   let sarA : gpu_array et (bm * bk) = fst sh;
-//   let sarB : gpu_array et (bk * bn) = fst (snd sh);
-//   rewrite each fst sh as sarA;
-//   rewrite each fst (snd sh) as sarB;
+// #push-options "--split_queries always --debug SMTFail"
+// #push-options "--z3rlimit 40 --retry 5"
+// #push-options "--print_implicits"
+inline_for_extraction noextract
+fn kf
+  (#et_ab #et_c : Type0)
+  {| scalar et_ab, scalar et_c |}
+  (#rows #shared #cols : szp)
+  (#lA : mlayout rows shared) {| clayout lA |}
+  (gA : gpu_matrix et_ab lA)
+  (#eA : ematrix et_ab rows shared)
+  (#lB : mlayout shared cols) {| clayout lB |}
+  (gB : gpu_matrix et_ab lB)
+  (#eB : ematrix et_ab shared cols)
+  (gC : gpu_matrix et_c (R.row_major rows cols))
+  (bm : szp{bm /? rows})
+  (bn : szp{bn /? cols})
+  (bk : szp{bk /? shared})
+  (#_: squash (SZ.fits (bm * bk) /\ SZ.fits (bk * bn)))
+  (tm : szp{tm /? bm})
+  (tn : szp{tn /? bn})
+  (tk : szp{tk /? bk})
+  (#_ : squash (SZ.fits (bm*bk + bm/tm*(bn/tn))))
+  (#_ : squash (SZ.fits (bk*bn + bm/tm*(bn/tn))))
+  (#fA #fB : perm)
+  (sh : c_shmems (shmems_desc et_ab bm bn bk))
+  (bid : szlt (rows/bm * (cols/bn)))
+  (tid : szlt (bm/tm * (bn/tn)))
+  ()
+  requires
+    gpu **
+    kpre gA eA gB eB gC bm bn bk tm tn tk fA fB sh bid tid **
+    thread_id (bm/tm * (bn/tn)) tid **
+    block_id (rows/bm * (cols/bn)) bid
+  ensures
+    gpu **
+    kpost (* comb *) gA eA gB eB gC bm bn bk tm tn fA fB sh bid tid **
+    thread_id (bm/tm * (bn/tn)) tid **
+    block_id (rows/bm * (cols/bn)) bid
+{
+  let sarA : gpu_array et_ab (bm * bk) = fst sh;
+  let sarB : gpu_array et_ab (bk * bn) = fst (snd sh);
+  rewrite each fst sh as sarA;
+  rewrite each fst (snd sh) as sarB;
 
-//   gpu_pts_to_ref sarA;
-//   gpu_pts_to_ref sarB;
+  gpu_pts_to_ref sarA;
+  gpu_pts_to_ref sarB;
+  // This leads to a faillure to resolve the clayout when calling populate_shmem
+  // let slA = R.row_major bm bk;
+  // assert (rewrites_to slA (R.row_major bm bk));
+  // let slB = R.row_major bk bn;
+  // assert (rewrites_to slB (R.row_major bk bn));
 
-//   unfold barrier_tok slA slB sarA sarB 0 (bm/tm * (bn/tn)) tid;
+  unfold barrier_tok (R.row_major bm bk) (R.row_major bk bn) sarA sarB 0 (bm/tm * (bn/tn)) tid;
 
-//   gpu_matrix_abs' slA sarA;
-//   let sA = from_array slA sarA;
-//   rewrite each from_array slA sarA as sA;
+  gpu_matrix_abs' (R.row_major bm bk) sarA;
+  let sA = from_array (R.row_major bm bk) sarA;
+  rewrite each from_array (R.row_major bm bk) sarA as sA;
 
-//   gpu_matrix_abs' slB sarB;
-//   let sB = from_array slB sarB;
-//   rewrite each from_array slB sarB as sB;
+  gpu_matrix_abs' (R.row_major bk bn) sarB;
+  let sB = from_array (R.row_major bk bn) sarB;
+  rewrite each from_array (R.row_major bk bn) sarB as sB;
 
-//   let num_k_tiles = shared /^ bk;
-//   let num_n_tiles = cols /^ bn;
-//   let mrow = bid /^ num_n_tiles;
-//   let mcol = bid %^ num_n_tiles;
+  let num_k_tiles = shared /^ bk;
+  let num_n_tiles = cols /^ bn;
+  let mrow = bid /^ num_n_tiles;
+  let mcol = bid %^ num_n_tiles;
 
-//   let threadRow = tid /^ (bn/^tn);
-//   let threadCol = tid %^ (bn/^tn);
+  let threadRow = tid /^ (bn/^tn);
+  let threadCol = tid %^ (bn/^tn);
 
-//   // (* tensor core fragments *)
-//   let aFrag = __alloc_fragment et FragA tm tn tk FragLRM;
-//   let bFrag = __alloc_fragment et FragB tm tn tk FragLRM;
-//   let accumFrag = __alloc_fragment et FragAccum tm tn tk FragAccum;
-//   mma_fill accumFrag fill_value_zero;
+  (* tensor core fragments *)
+  let aFrag = __alloc_fragment et_ab FragA tm tn tk FragLRM;
+  let bFrag = __alloc_fragment et_ab FragB tm tn tk FragLRM;
+  let accumFrag = __alloc_fragment et_c FragAcc tm tn tk FragLAcc;
 
-//   let mut bkIdx  : sz = 0sz;
-//   while (SZ.(!bkIdx <^ num_k_tiles))
-//     invariant
-//       exists* (vbkIdx : SZ.t{vbkIdx <= num_k_tiles})
-//         (vaFrag : ematrix half tm tk) (vbFrag : ematrix half tk tn) (vaccumFrag : ematrix half tm tn).
-//         bkIdx |-> vbkIdx **
-//         aFrag |-> vaFrag **
-//         bFrag |-> vbFrag **
-//         accumFrag |-> vaccumFrag
-//         (exists* (x : ematrix _ _ _). sA |-> Frac (1.0R /. ((bm/tm*(bn/tn)))) x) **
-//         (exists* (x : ematrix _ _ _). sB |-> Frac (1.0R /. ((bm/tm*(bn/tn)))) x) **
-//         B.barrier_tok (barrier_p sA sB ((bm/tm*(bn/tn)))) (barrier_q sA sB ((bm/tm*(bn/tn)))) (2 * vbkIdx) tid **
-//         gpu
-//   {
-//     (* This assert should not be needed. I don't know what effect it even has. *)
-//     let vbkIdx = !bkIdx;
-//     assert B.barrier_tok (barrier_p sA sB (bm/tm * (bn/tn))) (barrier_q sA sB (bm/tm * (bn/tn))) (2 * vbkIdx) tid;
-//     even_2x vbkIdx;
-//     rewrite
-//         (exists* (x : ematrix _ _ _). sA |-> Frac (1.0R /. (bm/tm * (bn/tn))) x) **
-//         (exists* (x : ematrix _ _ _). sB |-> Frac (1.0R /. (bm/tm * (bn/tn))) x)
-//       as barrier_p sA sB (bm/tm * (bn/tn)) (2 * vbkIdx) tid;
+  (* get ownership over the thread's gC tile and load it into the accumulator *)
+  unfold own_thread_tile gC bm bn tm tn bid tid;
+  let t_tile = thread_tile (block_tile gC (SZ.v bm) (SZ.v bn) (SZ.v bid)) (SZ.v tm) (SZ.v tn) (SZ.v tid);
+  assert (rewrites_to t_tile (thread_tile (block_tile gC (SZ.v bm) (SZ.v bn) (SZ.v bid)) (SZ.v tm) (SZ.v tn) (SZ.v tid)));
+  mma_loadAccum accumFrag t_tile;
+  fold own_thread_tile gC bm bn tm tn bid tid;
 
-//     B.barrier_wait ();
-//     rewrite (barrier_q sA sB (bm/tm * (bn/tn)) (2 * vbkIdx) tid)
-//         as own_tile_stride_cells sA (bm/tm * (bn/tn)) tid **
-//            own_tile_stride_cells sB (bm/tm * (bn/tn)) tid;
+  let mut bkIdx  : sz = 0sz;
+  while (SZ.(!bkIdx <^ num_k_tiles))
+    invariant
+      exists* (vbkIdx : SZ.t{vbkIdx <= num_k_tiles})
+        (vaFrag : ematrix et_ab tm tk) (vbFrag : ematrix et_ab tk tn) (vaccumFrag : ematrix et_c tm tn).
+        bkIdx |-> vbkIdx **
+        aFrag |-> vaFrag **
+        bFrag |-> vbFrag **
+        accumFrag |-> vaccumFrag **
+        (exists* (x : ematrix _ _ _). sA |-> Frac (1.0R /. ((bm/tm*(bn/tn)))) x) **
+        (exists* (x : ematrix _ _ _). sB |-> Frac (1.0R /. ((bm/tm*(bn/tn)))) x) **
+        B.barrier_tok (barrier_p sA sB ((bm/tm*(bn/tn)))) (barrier_q sA sB ((bm/tm*(bn/tn)))) (2 * vbkIdx) tid
+  {
+    (* This assert should not be needed. I don't know what effect it even has. *)
+    let vbkIdx = !bkIdx;
+    assert B.barrier_tok (barrier_p sA sB (bm/tm * (bn/tn))) (barrier_q sA sB (bm/tm * (bn/tn))) (2 * vbkIdx) tid;
+    even_2x vbkIdx;
+    assert pure((2 * vbkIdx % 2 = 0) == true);
+    rewrite
+        // WARNING after reintroducing the paranthesis in barrier_p, this checks
+        //  It seems that either there are paranthesis in both or in neither, otherwise the assertion fails
+        (exists* (x : ematrix _ _ _). sA |-> Frac (1.0R /. (bm/tm * (bn/tn))) x) **
+        (exists* (x : ematrix _ _ _). sB |-> Frac (1.0R /. (bm/tm * (bn/tn))) x)
+      as barrier_p sA sB (bm/tm * (bn/tn)) (2 * vbkIdx) tid;
 
-//     populate_shmem bm bn bk tm tn sA sB gA gB mrow !bkIdx mcol tid;
+    B.barrier_wait ();
+    rewrite (barrier_q sA sB (bm/tm * (bn/tn)) (2 * vbkIdx) tid)
+        as own_tile_stride_cells sA (bm/tm * (bn/tn)) tid **
+           own_tile_stride_cells sB (bm/tm * (bn/tn)) tid;
 
-//     assert (B.barrier_tok (barrier_p sA sB (bm/tm * (bn/tn))) (barrier_q sA sB (bm/tm * (bn/tn))) (2 * vbkIdx + 1) tid);
-//     odd_2x1 vbkIdx;
-//     assert (pure (odd (2 * vbkIdx + 1)));
-//     rewrite own_tile_stride_cells sA (bm/tm * (bn/tn)) tid **
-//             own_tile_stride_cells sB (bm/tm * (bn/tn)) tid
-//          as (barrier_p sA sB (bm/tm * (bn/tn)) (2 * vbkIdx + 1) tid);
+    populate_shmem bm bn bk tm tn sA sB gA gB mrow !bkIdx mcol tid;
 
-//     B.barrier_wait ();
+    assert (B.barrier_tok (barrier_p sA sB (bm/tm * (bn/tn))) (barrier_q sA sB (bm/tm * (bn/tn))) (2 * vbkIdx + 1) tid);
+    odd_2x1 vbkIdx;
+    assert (pure (odd (2 * vbkIdx + 1)));
+    rewrite own_tile_stride_cells sA (bm/tm * (bn/tn)) tid **
+            own_tile_stride_cells sB (bm/tm * (bn/tn)) tid
+         as (barrier_p sA sB (bm/tm * (bn/tn)) (2 * vbkIdx + 1) tid);
 
-//     even_2x (vbkIdx + 1);
-//     assert (pure (2 * (vbkIdx + 1) == 2 * vbkIdx + 2));
-//     assert (pure (even (2 * vbkIdx + 2)));
-//     rewrite (barrier_q sA sB (bm/tm * (bn/tn)) (2 * vbkIdx + 1) tid)
-//     as
-//       (exists* (x : ematrix _ _ _). sA |-> Frac (1.0R /. (bm/tm * (bn/tn))) x) **
-//       (exists* (x : ematrix _ _ _). sB |-> Frac (1.0R /. (bm/tm * (bn/tn))) x);
+    B.barrier_wait ();
 
-//     subproducts_tc bm bn bk tm tn tk aFrag bFrag accumFrag sA sB threadRow threadCol;
+    even_2x (vbkIdx + 1);
+    assert (pure (2 * (vbkIdx + 1) == 2 * vbkIdx + 2));
+    assert (pure (even (2 * vbkIdx + 2)));
+    rewrite (barrier_q sA sB (bm/tm * (bn/tn)) (2 * vbkIdx + 1) tid)
+    as
+      (exists* (x : ematrix _ _ _). sA |-> Frac (1.0R /. (bm/tm * (bn/tn))) x) **
+      (exists* (x : ematrix _ _ _). sB |-> Frac (1.0R /. (bm/tm * (bn/tn))) x);
 
-//     bkIdx := !bkIdx +^ 1sz;
-//   };
+    subproducts_tc bm bn bk tm tn tk aFrag bFrag accumFrag sA sB threadRow threadCol;
 
-//   epilogue comb bm bn tm tn accumFrag gC bid tid;
+    bkIdx := !bkIdx +^ 1sz;
+  };
 
-//   gpu_matrix_concr sA; rewrite each core sA as sarA;
-//   gpu_matrix_concr sB; rewrite each core sB as sarB;
+  epilogue bm bn tm tn accumFrag gC bid tid;
 
-//   fold barrier_tok slA slB sarA sarB (2 * num_k_tiles) (bm/tm * (bn/tn)) tid;
+  with vaFrag. assert aFrag |-> vaFrag; drop_ (aFrag |-> vaFrag);
+  with vbFrag. assert bFrag |-> vbFrag; drop_ (bFrag |-> vbFrag);
+  with vaccumFrag. assert accumFrag |-> vaccumFrag; drop_ (accumFrag |-> vaccumFrag);
 
-//   rewrite each sarA as fst sh;
-//   rewrite each sarB as fst (snd sh);
-//   ()
-// }
+  gpu_matrix_concr sA; rewrite each core sA as sarA;
+  gpu_matrix_concr sB; rewrite each core sB as sarB;
+
+  fold barrier_tok (R.row_major bm bk) (R.row_major bk bn) sarA sarB (2 * num_k_tiles) (bm/tm * (bn/tn)) tid;
+
+  rewrite each sarA as fst sh;
+  rewrite each sarB as fst (snd sh);
+  ()
+}
 
 ghost
 fn setup
-  (#et : Type0) {| scalar et |}
-  (comb : binop et)
+  (#et_ab #et_c : Type0)
+  {| scalar et_ab, scalar et_c |}
   (#rows #shared #cols : szp)
   (#lA : mlayout rows shared)
   (#lB : mlayout shared cols)
   (#lC : mlayout rows cols)
   {| clayout lA, clayout lB, clayout lC |}
-  (gA : gpu_matrix et lA)
-  (eA : ematrix et rows shared)
-  (gB : gpu_matrix et lB)
-  (eB : ematrix et shared cols)
-  (gC : gpu_matrix et lC)
-  (eC : ematrix et rows cols)
+  (gA : gpu_matrix et_ab lA)
+  (eA : ematrix et_ab rows shared)
+  (gB : gpu_matrix et_ab lB)
+  (eB : ematrix et_ab shared cols)
+  (gC : gpu_matrix et_c lC)
+  (eC : ematrix et_c rows cols)
   (bm : szp{bm /? rows})
   (bn : szp{bn /? cols})
   (bk : szp{bk /? shared})
@@ -706,6 +749,7 @@ fn setup
   (#_: squash (SZ.fits (rows * cols)))
   (tm : szp{tm /? bm})
   (tn : szp{tn /? bn})
+  (tk : szp{tk /? bk})
   (nblk : szp{SZ.v nblk == rows/bm * (cols/bn)})
   (nthr : szp{SZ.v nthr == bm/tm * (bn/tn)})
   (fA fB : perm)
@@ -718,7 +762,7 @@ fn setup
   ensures
     (forall+ (bid : natlt nblk)
              (tid : natlt nthr).
-      kpre1 comb gA eA gB eB gC bm bn bk tm tn fA fB bid tid) **
+      kpre1 (*comb*) gA eA gB eB gC bm bn bk tm tn tk fA fB bid tid) **
     emp (* frame *)
 {
   admit();
@@ -726,33 +770,32 @@ fn setup
 
 ghost
 fn block_setup
-  (#et : Type0) {| scalar et |}
-  (comb : binop et)
+  (#et_ab #et_c : Type0)
+  {| scalar et_ab, scalar et_c |}
   (#rows #shared #cols : szp)
   (#lA : mlayout rows shared)
   (#lB : mlayout shared cols)
   (#lC : mlayout rows cols)
-  (gA : gpu_matrix et lA)
-  (eA : ematrix et rows shared)
-  (gB : gpu_matrix et lB)
-  (eB : ematrix et shared cols)
-  (gC : gpu_matrix et lC)
-  (eC : ematrix et rows cols)
+  {| clayout lA, clayout lB, clayout lC |}
+  (gA : gpu_matrix et_ab lA)
+  (eA : ematrix et_ab rows shared)
+  (gB : gpu_matrix et_ab lB)
+  (eB : ematrix et_ab shared cols)
+  (gC : gpu_matrix et_c lC)
+  (eC : ematrix et_c rows cols)
   (bm : szp{bm /? rows})
   (bn : szp{bn /? cols})
   (bk : szp{bk /? shared})
   // (#_: squash (SZ.fits (bm * bk) /\ SZ.fits (bk * bn)))
   (#_: squash (SZ.fits (bm * bn)))
   (#_: squash (SZ.fits (rows * cols)))
-  (slA : full_mlayout bm bk)
-  (slB : full_mlayout bk bn)
-  {| clayout slA, clayout slB |}
   (tm : szp{tm /? bm})
   (tn : szp{tn /? bn})
+  (tk : szp{tk /? bk})
   (nblk : szp{SZ.v nblk == rows/bm * (cols/bn)})
   (nthr : szp{SZ.v nthr == bm/tm * (bn/tn)})
   (fA fB : perm)
-  (sh : c_shmems (shmems_desc et bm bn bk))
+  (sh : c_shmems (shmems_desc et_ab bm bn bk))
   (bid : natlt nblk)
   ()
   norewrite
@@ -760,11 +803,11 @@ fn block_setup
     block_setup_tok nthr **
     live_c_shmems sh **
     (forall+ (tid : natlt nthr).
-      kpre1 comb gA eA gB eB gC bm bn bk tm tn fA fB bid tid)
+      kpre1 (* comb *) gA eA gB eB gC bm bn bk tm tn tk fA fB bid tid)
   ensures
     block_setup_tok nthr **
     (forall+ (tid : natlt nthr).
-      kpre comb gA eA gB eB gC bm bn bk slA slB tm tn fA fB sh bid tid) **
+      kpre (* comb *) gA eA gB eB gC bm bn bk tm tn tk fA fB sh bid tid) **
     emp (* frame *)
 {
   admit();
@@ -772,62 +815,59 @@ fn block_setup
 
 ghost
 fn block_teardown
-  (#et : Type0) {| scalar et |}
-  (comb : binop et)
+  (#et_ab #et_c : Type0)
+  {| scalar et_ab, scalar et_c |}
   (#rows #shared #cols : szp)
   (#lA : mlayout rows shared)
   (#lB : mlayout shared cols)
   (#lC : mlayout rows cols)
-  (gA : gpu_matrix et lA)
-  (eA : ematrix et rows shared)
-  (gB : gpu_matrix et lB)
-  (eB : ematrix et shared cols)
-  (gC : gpu_matrix et lC)
-  (eC : ematrix et rows cols)
+  (gA : gpu_matrix et_ab lA)
+  (eA : ematrix et_ab rows shared)
+  (gB : gpu_matrix et_ab lB)
+  (eB : ematrix et_ab shared cols)
+  (gC : gpu_matrix et_c lC)
+  (eC : ematrix et_c rows cols)
   (bm : szp{bm /? rows})
   (bn : szp{bn /? cols})
   (bk : szp{bk /? shared})
-  // (#_: squash (SZ.fits (bm * bk) /\ SZ.fits (bk * bn)))
+  (#_: squash (SZ.fits (bm * bk) /\ SZ.fits (bk * bn)))
   (#_: squash (SZ.fits (rows * cols)))
   (#_: squash (SZ.fits (bm * bn)))
-  (slA : full_mlayout bm bk)
-  (slB : full_mlayout bk bn)
-  {| clayout slA, clayout slB |}
   (tm : szp{tm /? bm})
   (tn : szp{tn /? bn})
   (nblk : szp{SZ.v nblk == rows/bm * (cols/bn)})
   (nthr : szp{SZ.v nthr == bm/tm * (bn/tn)})
   (fA fB : perm)
-  (sh : c_shmems (shmems_desc et bm bn bk))
+  (sh : c_shmems (shmems_desc et_ab bm bn bk))
   (bid : natlt nblk)
   ()
   norewrite
   requires
     (forall+ (tid : natlt nthr).
-      kpost comb gA eA gB eB gC bm bn bk slA slB tm tn fA fB sh bid tid) **
+      kpost (* comb *) gA eA gB eB gC bm bn bk tm tn fA fB sh bid tid) **
     emp (* frame *)
   ensures
     live_c_shmems sh **
     (forall+ (tid : natlt nthr).
-      kpost1 comb gA eA gB eB gC bm bn bk tm tn fA fB bid tid)
+      kpost1 (* comb *) gA eA gB eB gC bm bn bk tm tn fA fB bid tid)
 {
   admit();
 }
 
 ghost
 fn teardown
-  (#et : Type0) {| scalar et |}
-  (comb : binop et)
+  (#et_ab #et_c : Type0)
+  {| scalar et_ab, scalar et_c |}
   (#rows #shared #cols : szp)
   (#lA : mlayout rows shared)
   (#lB : mlayout shared cols)
   (#lC : mlayout rows cols)
-  (gA : gpu_matrix et lA)
-  (eA : ematrix et rows shared)
-  (gB : gpu_matrix et lB)
-  (eB : ematrix et shared cols)
-  (gC : gpu_matrix et lC)
-  (eC : ematrix et rows cols)
+  (gA : gpu_matrix et_ab lA)
+  (eA : ematrix et_ab rows shared)
+  (gB : gpu_matrix et_ab lB)
+  (eB : ematrix et_ab shared cols)
+  (gC : gpu_matrix et_c lC)
+  (eC : ematrix et_c rows cols)
   (bm : szp{bm /? rows})
   (bn : szp{bn /? cols})
   (bk : szp{bk /? shared})
@@ -843,12 +883,14 @@ fn teardown
   requires
     (forall+ (bid : natlt nblk)
              (tid : natlt nthr).
-      kpre1 comb gA eA gB eB gC bm bn bk tm tn fA fB bid tid) **
+      kpost1 (* comb *) gA eA gB eB gC bm bn bk tm tn fA fB bid tid) **
     emp (* frame *)
   ensures
     gA |-> Frac fA eA **
     gB |-> Frac fB eB **
-    (gC |-> MS.mmcomb comb eC eA eB)
+    // underspec not implemented anyway
+    (exists* eC'. gC |-> eC')
+    // (gC |-> MS.mmcomb comb eC eA eB)
 {
   // forevery_flatten #(natlt2 mrows mcols) #_ #(natlt tile)
   //   (fun bid tid -> kpost1 comb tile gA gB gC eA eB 1.0R bid tid);
@@ -860,92 +902,85 @@ fn teardown
   admit();
 }
 
-// inline_for_extraction noextract
-// let mk_kernel
-//   (#et : Type0) {| scalar et |}
-//   (comb : binop et)
-//   (#rows #shared #cols : szp)
-//   (#lA : mlayout rows shared)
-//   (#lB : mlayout shared cols)
-//   (#lC : mlayout rows cols)
-//   {| clayout lA, clayout lB, clayout lC |}
-//   (gA : gpu_matrix et lA)
-//   (#eA : ematrix et rows shared)
-//   (gB : gpu_matrix et lB)
-//   (#eB : ematrix et shared cols)
-//   (gC : gpu_matrix et lC)
-//   (#eC : ematrix et rows cols)
-//   (bm : szp{bm /? rows})
-//   (bn : szp{bn /? cols})
-//   (bk : szp{bk /? shared})
-//   (#_: squash (SZ.fits (bm * bk) /\ SZ.fits (bk * bn)))
-//   (slA : full_mlayout bm bk)
-//   (slB : full_mlayout bk bn)
-//   {| clayout slA, clayout slB |}
-//   (tm : szp{tm /? bm})
-//   (tn : szp{tn /? bn})
-//   (#fA #fB : perm)
-//   (nblk : szp{SZ.v nblk == rows/bm * (cols/bn)})
-//   (nthr : szp{SZ.v nthr == bm/tm * (bn/tn)})
-//   (#_ : squash (SZ.fits (bm*bk + bm/tm*(bn/tn))))
-//   (#_ : squash (SZ.fits (bk*bn + bm/tm*(bn/tn))))
-//   (#_ : squash (rows/bm * (cols/bn) <= max_blocks
-//                /\ (bm/tm * (bn/tn)) <= max_threads))
-//   ()
-//   : kernel_desc
-//       (gA |-> Frac fA eA ** gB |-> Frac fB eB ** gC |-> eC)
-//       (gA |-> Frac fA eA ** gB |-> Frac fB eB ** (gC |-> MS.mmcomb comb eC eA eB))
-// = {
-//   nblk;// = rows/^bm *^ (cols/^bn);
-//   nthr;// = (bm /^ tm *^ (bn /^ tn));
+inline_for_extraction noextract
+let mk_kernel
+  (#et_ab #et_c : Type0)
+  {| scalar et_ab, scalar et_c |}
+  (#rows #shared #cols : szp)
+  (#lA : mlayout rows shared) {| clayout lA |}
+  (gA : gpu_matrix et_ab lA)
+  (#eA : ematrix et_ab rows shared)
+  (#lB : mlayout shared cols) {| clayout lB |}
+  (gB : gpu_matrix et_ab lB)
+  (#eB : ematrix et_ab shared cols)
+  (gC : gpu_matrix et_c (R.row_major rows cols))
+  (#_ : squash (SZ.fits (rows * cols)))
+  (#eC : ematrix et_c rows cols)
+  (bm : szp{bm /? rows})
+  (bn : szp{bn /? cols})
+  (bk : szp{bk /? shared})
+  (#_: squash (SZ.fits (bm * bk) /\ SZ.fits (bk * bn)))
+  (tm : szp{tm /? bm})
+  (tn : szp{tn /? bn})
+  (tk : szp{tk /? bk})
+  (#fA #fB : perm)
+  (nblk : szp{SZ.v nblk == rows/bm * (cols/bn)})
+  (nthr : szp{SZ.v nthr == bm/tm * (bn/tn)})
+  (#_ : squash (SZ.fits (bm*bk + bm/tm*(bn/tn))))
+  (#_ : squash (SZ.fits (bk*bn + bm/tm*(bn/tn))))
+  (#_ : squash (rows/bm * (cols/bn) <= max_blocks
+               /\ (bm/tm * (bn/tn)) <= max_threads))
+  ()
+  : kernel_desc
+      (gA |-> Frac fA eA ** gB |-> Frac fB eB ** gC |-> eC)
+      (gA |-> Frac fA eA ** gB |-> Frac fB eB ** (exists* eC'. gC |-> eC'))
+= {
+  nblk;// = rows/^bm *^ (cols/^bn);
+  nthr;// = (bm /^ tm *^ (bn /^ tn));
 
-//   shmems_desc = shmems_desc et bm bn bk;
+  shmems_desc = shmems_desc et_ab bm bn bk;
 
-//   frame = emp;
-//   block_pre  = (fun bid -> forall+ (tid : natlt nthr). kpre1  comb gA eA gB eB gC bm bn bk tm tn fA fB bid tid);
-//   block_post = (fun bid -> forall+ (tid : natlt nthr). kpost1 comb gA eA gB eB gC bm bn bk tm tn fA fB bid tid);
+  frame = emp;
+  block_pre  = (fun bid -> forall+ (tid : natlt nthr). kpre1  (* comb *) gA eA gB eB gC bm bn bk tm tn tk fA fB bid tid);
+  block_post = (fun bid -> forall+ (tid : natlt nthr). kpost1 (* comb *) gA eA gB eB gC bm bn bk tm tn fA fB bid tid);
 
-//   setup      = setup    comb gA eA gB eB gC eC bm bn bk tm tn nblk nthr fA fB;
-//   teardown   = teardown comb gA eA gB eB gC eC bm bn bk tm tn nblk nthr fA fB;
+  setup      = setup    (* comb *) gA eA gB eB gC eC bm bn bk tm tn tk nblk nthr fA fB;
+  teardown   = teardown (* comb *) gA eA gB eB gC eC bm bn bk tm tn nblk nthr fA fB;
 
-//   block_frame    = (fun _ar _bid -> emp);
-//   block_setup    = block_setup comb gA eA gB eB gC eC bm bn bk slA slB tm tn nblk nthr fA fB;
-//   block_teardown = block_teardown comb gA eA gB eB gC eC bm bn bk slA slB tm tn nblk nthr fA fB ;
+  block_frame    = (fun _ar _bid -> emp);
+  block_setup    = block_setup (* comb *) gA eA gB eB gC eC bm bn bk tm tn tk nblk nthr fA fB;
+  block_teardown = block_teardown (* comb *) gA eA gB eB gC eC bm bn bk tm tn nblk nthr fA fB ;
 
-//   kpre      = kpre  comb gA eA gB eB gC bm bn bk slA slB tm tn fA fB;
-//   kpost     = kpost comb gA eA gB eB gC bm bn bk slA slB tm tn fA fB;
+  kpre      = kpre  (* comb *) gA eA gB eB gC bm bn bk tm tn tk fA fB;
+  kpost     = kpost (* comb *) gA eA gB eB gC bm bn bk tm tn fA fB;
 
-//   f = kf comb gA #eA gB #eB gC bm bn bk slA slB tm tn #() #() #fA #fB;
-// }
-
-
+  f = kf (* comb *) gA #eA gB #eB gC bm bn bk tm tn tk #() #() #fA #fB;
+}
 
 inline_for_extraction noextract
 fn mmcomb_gpu
-  (#et : Type0) {| scalar et |}
-  (comb : binop et)
+  (#et_ab #et_c : Type0)
+  {| scalar et_ab, scalar et_c |}
   (#rows #shared #cols : szp)
   (#lA : mlayout rows shared)
   (#lB : mlayout shared cols)
-  (#lC : mlayout rows cols)
-  {| clayout lA, clayout lB, clayout lC |}
-  (gA : gpu_matrix et lA)
-  (#eA : ematrix et rows shared)
-  (gB : gpu_matrix et lB)
-  (#eB : ematrix et shared cols)
-  (gC : gpu_matrix et lC)
-  (#eC : ematrix et rows cols)
+  {| clayout lA, clayout lB |}
+  (gA : gpu_matrix et_ab lA)
+  (#eA : ematrix et_ab rows shared)
+  (gB : gpu_matrix et_ab lB)
+  (#eB : ematrix et_ab shared cols)
+  (gC : gpu_matrix et_c (R.row_major rows cols))
+  (#_ : squash (SZ.fits (rows * cols)))
+  (#eC : ematrix et_c rows cols)
   (bm : szp{bm /? rows})
   (bn : szp{bn /? cols})
   (bk : szp{bk /? shared})
   (tm : szp{tm /? bm})
   (tn : szp{tn /? bn})
+  (tk : szp{tk /? bk})
   (#_ : squash (SZ.fits (bm*bk + bm/tm*(bn/tn))))
   (#_ : squash (SZ.fits (bk*bn + bm/tm*(bn/tn))))
   (#_: squash (SZ.fits (bm * bk) /\ SZ.fits (bk * bn)))
-  (slA : full_mlayout bm bk)
-  (slB : full_mlayout bk bn)
-  {| clayout slA, clayout slB |}
   (#fA #fB : perm)
   norewrite
   preserves
@@ -957,10 +992,7 @@ fn mmcomb_gpu
     pure (bm/tm * (bn/tn) <= max_threads) **
     gC |-> eC
   ensures
-    gC |-> MS.mmcomb comb eC eA eB
+    (exists* eC'. gC |-> eC')
 {
-  (* fixed the inner layouts, or we'd have to propagate this everywhere? *)
-  // launch_sync (mk_kernel comb gA gB gC bm bn bk slA slB tm tn (rows/^bm *^ (cols/^bn)) (bm/^tm *^ (bn/^tn)) ());
-  admit();
+  launch_sync (mk_kernel gA gB gC bm bn bk tm tn tk (rows/^bm *^ (cols/^bn)) (bm/^tm *^ (bn/^tn)) ());
 }
-
